fixed structure of the proof, removed some admits in switch, deleted deprecated files

src/C_strtoimax/VstProof/VstSpec.v
@@ -1,62 +1,113 @@
 (* VST specification of asn_strtoimax_lim *)
 Require Import Clight.INTEGER.
-
-
-Require Import Spec2.
 Require Import Core.Core Core.Tactics Core.PtrLemmas.
-Require Import StructTact.StructTactics.
+Require Import StructTact.StructTactics Psatz.
 Require Import VST.floyd.proofauto.
 Definition Vprog : varspecs. mk_varspecs prog. Defined.
 Instance CompSpecs : compspecs. make_compspecs prog. Defined.
 
-Section VstStrtoimaxSpec.
+Require Import AbstractSpec.
 
- Definition asn_strtoimax_lim_vst_spec : ident * funspec :=
+Section VstSpec.
+
+Definition asn_strtoimax_lim_vst_spec : ident * funspec :=
   DECLARE _asn_strtoimax_lim
-    WITH str_b : block, str_ofs : ptrofs,
-         (* points at the start of the string *)
-         end_b : block, end_ofs : ptrofs,
-         (* points at the end of the string *)
+    (* WITH: binds variables in Pre- and Postconditions *)
+    WITH (* start of the string str *)
+         str_b : block, str_ofs : ptrofs,
+         (* end of the string *end *)
          end'_b : block, end'_ofs : ptrofs,
-         (* points at the last character in the string *)
+         (* stores address of the end of the string end *)
+         end_b : block, end_ofs : ptrofs,
+         (* stores result intp *)
          intp_b : block, intp_ofs : ptrofs,
-         (* pointers to store result in *)
-         sh_s : share, sh_e : share, sh_r : share,
-         (* string share, end share, result share *)
-         con : list Z, ch : val, res : val                           
-         (* contents, char at the end of string, initial value of intp *)
-    PRE [_str OF (tptr tschar), _end OF (tptr (tptr tschar)), _intp OF (tptr tlong)]
-      PROP(readable_share sh_s; writable_share sh_e; writable_share sh_r;
-           str_b = end'_b;
-           Zlength con = Z.max 0 (Ptrofs.unsigned end'_ofs - Ptrofs.unsigned str_ofs))
-      LOCAL(temp _str (Vptr str_b str_ofs);
-            temp _end (Vptr end_b end_ofs); 
-            temp _intp (Vptr intp_b intp_ofs))
-      SEP(if (Ptrofs.unsigned str_ofs <? Ptrofs.unsigned end'_ofs) 
-          then data_at sh_s (tarray tschar (Zlength con)) 
-                       (map Vbyte (map Byte.repr con)) (Vptr str_b str_ofs) * 
-               data_at sh_e (tptr tschar) (Vptr end'_b end'_ofs) (Vptr end_b end_ofs) * 
-               data_at sh_s tschar ch (Vptr end'_b end'_ofs)
-          else valid_pointer (Vptr str_b str_ofs) * 
-               valid_pointer (Vptr end'_b end'_ofs) *
-               data_at sh_e (tptr tschar) (Vptr end'_b end'_ofs) (Vptr end_b end_ofs);
-          data_at sh_r tint res (Vptr intp_b intp_ofs))
-    POST [tint]
-      PROP()
-      LOCAL(temp ret_temp (Vint (asn_strtox_result_e_to_int 
-                                   (return_type 
-                                      (asn_strtoimax_lim_spec con)))))
-      SEP(if (Ptrofs.unsigned str_ofs <? Ptrofs.unsigned end'_ofs) 
-          then data_at sh_s (tarray tschar (Zlength con)) 
-                       (map Vbyte (map Byte.repr con)) (Vptr str_b str_ofs) * 
-               data_at sh_e (tptr tschar) (Vptr end'_b end'_ofs) (Vptr end_b end_ofs) * 
-               data_at sh_s tschar ch (Vptr end'_b end'_ofs)
-          else valid_pointer (Vptr str_b str_ofs) * 
-               valid_pointer (Vptr end'_b end'_ofs) *
-               data_at sh_e (tptr tschar) (Vptr end'_b end'_ofs) (Vptr end_b end_ofs);
-          data_at sh_r tint res (Vptr intp_b intp_ofs)).
+         (* permission shares, cf. Verifiable C book (p.73) *)
+         sh_str : share, sh_end : share, sh_intp : share,
+         (* input string *)
+         contents : list byte,
+         (* contents of intp *)
+         v : val
+    (* Preconditions *)
+    (* Type declaration for parameters of the function *)
+    PRE [ _str OF (tptr tschar),
+          _end OF (tptr (tptr tschar)),
+          _intp OF (tptr tlong) ]
+    (* PROP: Propositions (of type Prop) that should hold
+       before executing the function. ; is conjuction *)
+      PROP ( (* Permissions for memory access *)
+          readable_share sh_str;  (* str points to readable memory *)
+          writable_share sh_end;  (* end points to writable memory *)
+          writable_share sh_intp; (* intp points to writable memory *)
 
-End VstStrtoimaxSpec.
+          (* str and end' should point to the same object, 
+           otherwise incomparable by C standard *)
+          str_b = end'_b;
+
+          (* length of contents = distance between str and end' *)
+          Zlength contents =
+          Z.max 0 (Ptrofs.unsigned end'_ofs - Ptrofs.unsigned str_ofs))
+      (* LOCAL: connects C light prameter identifiers and declared variables *)
+      LOCAL (temp _str (Vptr str_b str_ofs);
+             temp _end (Vptr end_b end_ofs); 
+             temp _intp (Vptr intp_b intp_ofs))
+      (* SEP: Propositions about memory (of type mem -> Prop (mpred)) that 
+         should hold before executing the function. 
+         ; (and * ) is separating conjunction, && is ordinary conjuction *)
+      SEP ((* str and end' are comparable, i.e. point within the same object *)
+           valid_pointer (Vptr end'_b end'_ofs) ;
+           valid_pointer (Vptr str_b str_ofs) ;
+           (* str points to contents with readable permission *)
+           data_at sh_str (tarray tschar (Zlength contents)) 
+                   (map Vbyte contents) (Vptr str_b str_ofs) ; 
+           (* end points to end' with writable permission *)
+           data_at sh_end (tptr tschar) (Vptr end'_b end'_ofs) 
+                   (Vptr end_b end_ofs);
+           (* intp points to some value v  *)
+           data_at sh_intp (tlong) v (Vptr intp_b intp_ofs))     
+    (* Postconditions *)
+    (* Type declaration for return value of the function *)
+    POST [tint]
+      (* No new propositions hold after executing the function *)
+      PROP()
+      (* Return value of the function corresponds to the result 
+         of abstract spec on contents *)
+      LOCAL (temp ret_temp (Vint (asn_strtox_result_e_to_int 
+                                   (res 
+                                      (Z_of_string contents)))))
+      (* Propositions about memory that hold after executing the function *)
+      SEP( (* this part didn't change after execution *) 
+           
+           valid_pointer (Vptr end'_b end'_ofs) ;
+           valid_pointer (Vptr str_b str_ofs) ;
+           data_at sh_str (tarray tschar (Zlength contents)) 
+                   (map Vbyte contents) (Vptr str_b str_ofs) ;
+           let r := res (Z_of_string contents) in
+            (* in 3 cases intp stays unchanged,
+              otherwise store the end value of Z_of_string *)
+            match r with 
+              | ASN_STRTOX_ERROR_RANGE 
+              | ASN_STRTOX_ERROR_INVAL 
+              | ASN_STRTOX_EXPECT_MORE => 
+                data_at sh_intp (tlong) v (Vptr intp_b intp_ofs)
+              | _ => data_at sh_intp (tlong) 
+                         (Vlong (Int64.repr (value (Z_of_string contents))))
+                         (Vptr intp_b intp_ofs) 
+            end ;
+           (* if str >= end, end doesn't change, 
+              otherwise store the address of the last char read 
+              (before going out of range, reading extra data 
+              or successfully terminating) *)
+            let i := index (Z_of_string contents) in
+            if (Ptrofs.unsigned str_ofs <? Ptrofs.unsigned end'_ofs)
+            then data_at sh_end (tptr tschar) 
+                         (Vptr str_b (Ptrofs.add str_ofs (Ptrofs.repr i))) 
+                         (Vptr end_b end_ofs)
+            else data_at sh_end (tptr tschar) (Vptr end'_b end'_ofs) 
+                         (Vptr end_b end_ofs)).
+
+End VstSpec.
+
+(* Proof *)
 
 Lemma typed_true_ptr_ge : forall b ptr1 ptr2, 
     typed_true tint (force_val (sem_cmp_pp Cge (Vptr b ptr1) (Vptr b ptr2))) ->
@@ -84,106 +135,294 @@ Proof.
   Lia.lia.
 Qed.
 
+(* Proposition data_at_array_valid_pointer *)
+
 Arguments valid_pointer p : simpl never.
+
+Lemma extend_weak_valid_pointer : forall b ofs P, 
+    valid_pointer (Vptr b ofs) * P |-- weak_valid_pointer (Vptr b ofs).
+Proof.
+  intros.
+  pose proof valid_pointer_weak (Vptr b ofs).
+  apply derives_trans with (Q := valid_pointer (Vptr b ofs)).
+  entailer!.
+  eassumption.
+Qed.
+
 
 Definition Gprog := ltac:(with_library prog [asn_strtoimax_lim_vst_spec]).
 
-Lemma body_asn_strtoimax_lim : semax_body Vprog Gprog f_asn_strtoimax_lim  asn_strtoimax_lim_vst_spec.
+Lemma body_asn_strtoimax_lim : semax_body Vprog Gprog f_asn_strtoimax_lim
+                                          asn_strtoimax_lim_vst_spec.
 Proof.
   start_function.
   rename H into EQB.
   rename H0 into LEN.
-  forward.
-  forward.
-  forward.
-  entailer!; inversion H1; inversion H3.
-  forward.
-  entailer!; inversion H1; inversion H3.
+  all: repeat forward; try entailer!.
+  1-2: break_and; inversion H7.
+
   destruct Z.ltb eqn:IFCON.
-  all: Intros.
-  all: forward.
-  all: forward_if.
-  all: try apply Z.ltb_lt in IFCON.
-  all: try apply Z.ltb_ge in IFCON.
-  
   - (* str < end' = true *)
-    (* Valid pointer proof *)
-    unfold test_order_ptrs; simpl.
-    destruct peq; [simpl|contradiction].
+    all: Intros.
 
-    apply andp_right.
-    *
+    forward_if; apply Z.ltb_lt in IFCON.
+    + (* Valid pointer proof *)
+      { unfold test_order_ptrs; simpl.
+        destruct peq; [simpl|contradiction].
+        apply andp_right.
+        apply derives_trans with (Q := valid_pointer (Vptr end'_b str_ofs)).
+        entailer!.
+        apply valid_pointer_weak.
+        apply derives_trans with (Q := valid_pointer (Vptr end'_b end'_ofs)).
+        entailer!.
+        apply valid_pointer_weak. }
+    + (*  srt >= end' from forward_if : contradiction *)
+      forward.
+      apply typed_true_ptr_ge in H.
+      rewrite Z.geb_le in H; Lia.lia.
+    + (*  str < end' = true from forward_if, go further in the branch *)
+      subst; apply typed_false_ptr_ge in H.
+      rewrite Z.gtb_lt in H.
+      assert (0 < Ptrofs.unsigned end'_ofs - Ptrofs.unsigned str_ofs)
+        by Lia.lia.
+      destruct contents.
+      replace (Zlength []) with (0) in LEN by reflexivity.
+      Lia.lia.
+      rewrite semax_lemmas.cons_app in LEN.
+      rewrite semax_lemmas.cons_app with (x := i).
+      rewrite Zlength_app in LEN.
+      assert (Zlength [i] = 1) as SING by reflexivity.
+      assert (Zlength contents = (Ptrofs.unsigned end'_ofs - 
+                                 Ptrofs.unsigned str_ofs) - 1) by lia.
+      rename H1 into LEN2.
+      assert (Zlength (map Vbyte [i]) = 1) as SINGB by reflexivity.
+      assert (Zlength (map Vbyte contents) = Zlength contents) 
+        as LENB by (apply Zlength_map); rewrite LEN2 in LENB.
+      rewrite <-Zlength_app in LEN; rewrite LEN; rewrite map_app.
+      rewrite split2_data_at_Tarray_app with (mid := 1) ; [|try eassumption | admit].
+      Intros.
+      rename v into v0.
+      assert (map Vbyte [i] = [Vbyte i]) as T by reflexivity.
+      pose proof data_at_singleton_array_eq (sh_str) (tschar) (Vbyte i) 
+           (map Vbyte [i]) (Vptr end'_b str_ofs) T as T1; rewrite T1; clear T T1.
+      forward.
+      forward.
+      normalize.
+      pose (sep_precondition := valid_pointer (Vptr end'_b end'_ofs) *
+                                valid_pointer (Vptr end'_b str_ofs) *
+                                data_at sh_str tschar (Vbyte i) (Vptr end'_b str_ofs) *
+                                data_at sh_str (tarray tschar 
+                                                       (Ptrofs.unsigned end'_ofs - 
+                                                        Ptrofs.unsigned str_ofs - 1))
+                                        (map Vbyte contents)
+                                        (field_address0 (tarray tschar 
+                                                                (Ptrofs.unsigned end'_ofs - 
+                                                                 Ptrofs.unsigned str_ofs))
+                                                        [ArraySubsc 1] (Vptr end'_b str_ofs)) *
+                                data_at sh_end (tptr tschar) (Vptr end'_b end'_ofs) 
+                                        (Vptr end_b end_ofs) *
+                                data_at sh_intp tlong v0 (Vptr intp_b intp_ofs)).
+      forward_if (
+          if Byte.signed i =? 45
+          then PROP()
+                   LOCAL( temp _sign (Vint (Int.repr (-1)));
+                          (if (Ptrofs.unsigned str_ofs + 1 <? Ptrofs.unsigned end'_ofs)
+                           then temp _str (Vptr end'_b (Ptrofs.add str_ofs (Ptrofs.repr 1)))
+                           else temp ret_temp (Vint (Int.repr (-1)))))
+                   SEP(sep_precondition)
+          else if Byte.signed i =? 43
+               then PROP()
+                        LOCAL( (if (Ptrofs.unsigned str_ofs + 1 <? Ptrofs.unsigned end'_ofs)
+                                then temp _str (Vptr end'_b (Ptrofs.add str_ofs (Ptrofs.repr 1)))
+                                else temp ret_temp (Vint (Int.repr (-1)))))
+                        SEP(sep_precondition)
+
+               else PROP()
+                        LOCAL()
+                        SEP(sep_precondition)). 
+      * (* if *str = '-' = Int.repr 45 *)
+        forward.
+        entailer!.
+        { replace (Int64.repr 0) with (Int64.zero) by reflexivity; 
+            replace (Int64.repr 1) with (Int64.one) by reflexivity.
+          rewrite Int64.not_zero.
+          unfold Int64.mods, Int64.shru, Z.shiftr.
+          rewrite Int64.unsigned_mone, Int64.unsigned_one; simpl.
+          repeat rewrite Int64.signed_repr;
+            unfold Int64.min_signed, Int64.max_signed;
+            unfold Int64.half_modulus, Int64.modulus;
+            cbn; Lia.lia. }
+        repeat forward.
+        forward_if.
+        ** unfold test_order_ptrs; simpl.
+           destruct peq; [simpl|contradiction].
+           apply andp_right.
+           admit.
+           apply derives_trans with (Q := valid_pointer (Vptr end'_b end'_ofs)).
+           entailer!.
+           apply valid_pointer_weak.
+           (* end_ofs <= str_ofs + 1, return EXPECT_MORE *)
+        ** repeat forward.
+           rename H1 into IFCON2.
+           apply typed_true_ptr_ge in IFCON2.
+           replace (Ptrofs.add str_ofs (Ptrofs.mul (Ptrofs.repr 1) 
+                                                   (Ptrofs.of_ints (Int.repr 1))))
+             with (Ptrofs.add str_ofs Ptrofs.one) in * by auto with ptrofs.
+           apply Z.geb_le in IFCON2.
+           replace (Ptrofs.unsigned (Ptrofs.add str_ofs Ptrofs.one)) 
+             with (Ptrofs.unsigned str_ofs + 1) in *. (* follows from IFCON *)
+           assert (Ptrofs.unsigned end'_ofs - Ptrofs.unsigned str_ofs - 1 = 0) as Z 
+               by nia.
+           assert (contents = []) as CONTENT.
+           rewrite Z in LEN2.
+           apply Zlength_nil_inv; assumption.
+           rewrite CONTENT.
+           unfold is_sign, plus_char, minus_char.
+           assert (Byte.eq i (Byte.repr 45) = true) as IS.
+           erewrite Byte.eq_signed.
+           break_if; auto.
+           rewrite IS; simpl.
+           replace (Byte.eq i (Byte.repr 43) || true)%bool with true by intuition.
+           simpl.
+           entailer!.
+           assert (map Vbyte [i] = [Vbyte i]) as T by reflexivity.
+           rewrite <-T; rewrite SING.
+           pose proof data_at_singleton_array_eq (sh_str) (tschar) (Vbyte i) 
+                (map Vbyte [i]) (Vptr end'_b str_ofs) T as T1; rewrite T1; clear T T1. 
+           entailer!.
+           replace (Ptrofs.unsigned end'_ofs - Ptrofs.unsigned str_ofs - 1) with 0.
+           apply data_at_zero_array_inv; simpl; reflexivity.
+           admit. (* Need to add precondition about str_ofs + Zlength contents <= Ptrofs.unsigned_max *)
+        ** (* str_ofs + 1 < end_ofs *)
+          forward.
+          rename H1 into IFCON2.
+          subst.
+          apply typed_false_ptr_ge in IFCON2.
+          replace (Ptrofs.add str_ofs (Ptrofs.mul (Ptrofs.repr 1) 
+                                                  (Ptrofs.of_ints (Int.repr 1))))
+            with (Ptrofs.add str_ofs Ptrofs.one) in * by auto with ptrofs.
+          rewrite Z.gtb_lt in IFCON2.
+          replace (Ptrofs.unsigned (Ptrofs.add str_ofs Ptrofs.one)) 
+            with (Ptrofs.unsigned str_ofs + 1) in *. (* follows from IFCON *)
+          rewrite E.
+          replace (Ptrofs.unsigned str_ofs + 1 <? Ptrofs.unsigned end'_ofs)
+            with true.
+          unfold sep_precondition. entailer!.
+          admit.
+          admit.
+      * (* if *str = '+' *)
+        repeat forward.
+        forward_if.
+        admit.
+        repeat forward.
+        entailer!.
+        normalize.
+        eapply typed_true_ptr_ge in H1.
+        replace  (Ptrofs.add str_ofs (Ptrofs.mul (Ptrofs.repr 1) (Ptrofs.of_ints (Int.repr 1))))
+          with  (Ptrofs.add str_ofs (Ptrofs.repr 1)) in * by auto with ptrofs.
+        assert (contents = []) as N.
+        eapply Z.geb_le in H1.
+        replace (Ptrofs.unsigned (Ptrofs.add str_ofs (Ptrofs.repr 1)))
+          with (Ptrofs.unsigned str_ofs + 1) in * by admit. (* follows from IFCON *)
+        assert (Ptrofs.unsigned end'_ofs - Ptrofs.unsigned str_ofs - 1 = 0) as Z by nia.
+        
+        autorewrite with sublist in *|-.
+        rewrite Z in LEN2.
+        Search Zlength [].
+        apply Zlength_nil_inv.
+        assumption.
+        rewrite N.
+        unfold is_sign, plus_char, minus_char.
+        assert (Byte.eq i (Byte.repr 43) = true) as IS.
+        Search Byte.eq.
+        erewrite Byte.eq_signed.
+        break_if; auto.
+        rewrite IS; simpl.
+        replace (true || Byte.eq i (Byte.repr 45))%bool with true.
+        reflexivity.
+        reflexivity.
+        normalize.
+        eapply typed_true_ptr_ge in H1.
+        replace  (Ptrofs.add str_ofs (Ptrofs.mul (Ptrofs.repr 1) (Ptrofs.of_ints (Int.repr 1))))
+          with  (Ptrofs.add str_ofs (Ptrofs.repr 1)) in * by auto with ptrofs.
+        assert (contents = []) as N.
+        eapply Z.geb_le in H1.
+        replace (Ptrofs.unsigned (Ptrofs.add str_ofs (Ptrofs.repr 1)))
+          with (Ptrofs.unsigned str_ofs + 1) in * by admit. (* follows from IFCON *)
+        assert (Ptrofs.unsigned end'_ofs - Ptrofs.unsigned str_ofs - 1 = 0) as Z by nia.
+        
+        autorewrite with sublist in *|-.
+        rewrite Z in LEN2.
+        apply Zlength_nil_inv.
+        assumption.
+        rewrite N.
+        unfold is_sign, plus_char, minus_char.
+        assert (Byte.eq i (Byte.repr 43) = true) as IS.
+        erewrite Byte.eq_signed.
+        break_if; auto.
+        rewrite IS; simpl.
+        replace (true || Byte.eq i (Byte.repr 45))%bool with true.
+        simpl.
+        entailer.
+        erewrite data_at_singleton_array_eq.
+        instantiate (1 :=  (Vbyte i)).
+        entailer!.
+        rewrite <- H14.
+        autorewrite with sublist.
+        rewrite data_at_zero_array_eq.
+        entailer!.
+        all: try auto.
+        
+        forward.
+        rewrite E.
+        replace (43 =? 45) with false by reflexivity.
+        replace (43 =? 43) with true by reflexivity.
+        replace (Ptrofs.unsigned str_ofs + 1 <? Ptrofs.unsigned end'_ofs)
+          with true.
+        unfold sep_precondition. entailer!.
+        admit.    
+      * (* default case *) 
+        forward.
+        replace (Byte.signed i =? 45) with false.
+        replace (Byte.signed i =? 43) with false.
+        unfold sep_precondition. entailer.
+        admit.
+        admit.
+        admit.
+      * (* Loop *)
+        repeat break_if.
+        (* case sign = -1 *)
+        Intros.
+        forward.
+        all: admit.
+  
+  - (* str >= end *)
+    all: try apply Z.ltb_ge in IFCON.
+    forward_if.
+    (* Valid pointer proof *)
+    { unfold test_order_ptrs; simpl.
+      destruct peq; [simpl|contradiction].
+      apply andp_right.
+      * apply derives_trans with (Q := valid_pointer (Vptr end'_b str_ofs)).
+        entailer!.
+        apply valid_pointer_weak.
+      * apply derives_trans with (Q := valid_pointer (Vptr end'_b end'_ofs)).
+        entailer!.
+        apply valid_pointer_weak. }
+
+    + (* str >= end, return INVAL *)
+      forward.
+      try apply Z.ltb_ge in IFCON.
       autorewrite with sublist in *|-.
-      (* follows from LEN and IFCON *)
-      assert (data_at sh_s (tarray tschar (Zlength con)) 
-                      (map Vbyte (map Byte.repr con)) (Vptr end'_b str_ofs) * 
-              data_at sh_e (tptr tschar) (Vptr end'_b end'_ofs) 
-                      (Vptr end_b end_ofs) * 
-              data_at sh_s tschar ch (Vptr end'_b end'_ofs) * 
-              data_at sh_r tint res (Vptr intp_b intp_ofs) 
-                      |-- valid_pointer (Vptr end'_b str_ofs)) by entailer!.
-      pose proof valid_pointer_weak (Vptr end'_b str_ofs).
-      apply derives_trans with (Q := valid_pointer (Vptr end'_b str_ofs)).
-      all: assumption.
-    *
-      assert (data_at sh_s (tarray tschar (Zlength con)) 
-                      (map Vbyte (map Byte.repr con)) (Vptr end'_b str_ofs) * 
-              data_at sh_e (tptr tschar) (Vptr end'_b end'_ofs) 
-                      (Vptr end_b end_ofs) * 
-              data_at sh_s tschar ch (Vptr end'_b end'_ofs) * 
-              data_at sh_r tint res (Vptr intp_b intp_ofs) 
-                      |-- valid_pointer (Vptr end'_b end'_ofs)) 
-        by entailer!.
-      pose proof valid_pointer_weak (Vptr end'_b end'_ofs).
-      apply derives_trans with (Q := valid_pointer (Vptr end'_b end'_ofs)).
-      all: assumption.
-
-  - (* str < end' = true || end' <= str = true (from forward_if) *)
-    forward.
-    apply typed_true_ptr_ge in H.
-    rewrite Z.geb_le in H; Lia.lia.
-
-  - (* str < end' = true || str < end' = true (from forward_if) *)
-    rewrite EQB in H; apply typed_false_ptr_ge in H.
-    rewrite Z.gtb_lt in H.
-    autorewrite with sublist in *|-.
-    assert (0 < Ptrofs.unsigned end'_ofs - Ptrofs.unsigned str_ofs)
-      by Lia.lia.
-    admit.
-
-  - (* end' <= str = true *)
-    (* Valid pointer proof *)
-    unfold test_order_ptrs; simpl.
-    destruct peq; [simpl|contradiction].
-
-    apply andp_right.
-    * 
-      assert (valid_pointer (Vptr end'_b str_ofs) * 
-              valid_pointer (Vptr end'_b end'_ofs) * 
-              data_at sh_e (tptr tschar) (Vptr end'_b end'_ofs) 
-                      (Vptr end_b end_ofs) * 
-              data_at sh_r tint res (Vptr intp_b intp_ofs) 
-                      |-- valid_pointer (Vptr end'_b str_ofs)) by entailer!.
-      pose proof valid_pointer_weak (Vptr end'_b str_ofs).
-      apply derives_trans with (Q := valid_pointer (Vptr end'_b str_ofs)).
-      all: assumption.
-    *
-      assert (valid_pointer (Vptr end'_b str_ofs) * 
-              valid_pointer (Vptr end'_b end'_ofs) * 
-              data_at sh_e (tptr tschar) (Vptr end'_b end'_ofs) 
-                      (Vptr end_b end_ofs) * 
-              data_at sh_r tint res (Vptr intp_b intp_ofs) 
-                      |-- valid_pointer (Vptr end'_b end'_ofs)) by entailer!.
-      pose proof valid_pointer_weak (Vptr end'_b end'_ofs).
-      apply derives_trans with (Q := valid_pointer (Vptr end'_b end'_ofs)).
-      all: assumption.
-
-  - (* end' <= str = true || end' <= str = true (from forward_if) *)
-    forward.
-    autorewrite with sublist in *|-.
-    pose proof Zlength_nil_inv con LEN as NIL.
-    rewrite NIL; simpl; entailer!.
-  - (* end' <= str = true || str < end' = true (from forward_if) *)
-    rewrite EQB in H; apply typed_false_ptr_ge in H.
-    rewrite Z.gtb_lt in H; Lia.lia.
+      try apply Z.ltb_ge in IFCON.
+      assert ((Ptrofs.unsigned end'_ofs - Ptrofs.unsigned str_ofs) <= 0)
+             by nia.
+      assert (Zlength contents = 0) as L by admit.
+      subst.
+      pose proof Zlength_nil_inv contents L as NIL.
+      rewrite NIL; simpl; entailer!.
+    +  (* end' <= str = true || str < end' = true (from forward_if) *)
+      try apply Z.ltb_lt in IFCON.
+      rewrite EQB in H; apply typed_false_ptr_ge in H.
+      rewrite Z.gtb_lt in H. lia.
 Admitted.
